javascript/javascriptAstScript.sml
@@ -26,8 +26,8 @@ val js_exp_def = Datatype `
 		| JSObjectRetrieve js_exp js_varN
     | JSBop js_binary_op js_exp js_exp
 		| JSVar js_varN
-		| JSAFun (js_varN list) js_exp
-		| JSFun js_varN (js_varN list) js_exp
+		| JSAFun (js_varN list) (js_exp list)
+		| JSFun js_varN (js_varN list) (js_exp list)
 		| JSApp js_exp (js_exp list)`;
 
 val js_stm_def = Datatype `
